feat: added proofs for decidability of whitespace and digits

Proofs/Helpers/Whitespace.v
@@ -9,24 +9,38 @@ Import ARM8Notations.
 
 Open Scope N.
 
-(* (0x09 <= b /\ b <= 0x0d) \/ b = 0x20 *)
-Inductive whitespace : N -> Prop :=
-  | whitespace_tab  : whitespace 0x9
-  | whitespace_lf   : whitespace 0xa
-  | whitespace_vt   : whitespace 0xb
-  | whitespace_ff   : whitespace 0xc
-  | whitespace_cf   : whitespace 0xd
-  | whitespace_dle  : whitespace 0x20.
-
-Fixpoint handle_whitespace (mem:memory) (p:addr) (k:nat) :=
-  match k with
-  | O => p (* return the mem val where theres no more whitespace *)
-  | S k' => 
-    match mem Ⓑ[p] with
-    | whitespace => handle_whitespace mem (p+1) k' (* move to next place *)
-    end
-  end.
-
 (* A byte is whitespace: 0x09-0x0d (tab through carriage return) or 0x20 (space) *)
 Definition is_whitespace (b : N) : Prop :=
   (0x09 <= b /\ b <= 0x0d) \/ b = 0x20.
+
+(* Boolean version for decidability *)
+Definition is_whitespace_b (b : N) : bool :=
+  ((0x09 <=? b) && (b <=? 0x0d)) || (b =? 0x20).
+
+(* Decidability lemma for is_whitespace *)
+Lemma is_whitespace_dec : forall b, {is_whitespace b} + {~is_whitespace b}.
+Proof.
+  intro b.
+  destruct (is_whitespace_b b) eqn:Hb.
+  - left. unfold is_whitespace, is_whitespace_b in *.
+    apply Bool.orb_true_iff in Hb. destruct Hb as [Hb|Hb].
+    + left. apply Bool.andb_true_iff in Hb. destruct Hb as [H1 H2].
+      apply N.leb_le in H1. apply N.leb_le in H2. split; assumption.
+    + right. apply N.eqb_eq in Hb. assumption.
+  - right. unfold is_whitespace, is_whitespace_b in *.
+    apply Bool.orb_false_iff in Hb. destruct Hb as [Hb1 Hb2].
+    intros [H|H].
+    + destruct H as [H1 H2]. apply Bool.andb_false_iff in Hb1.
+      destruct Hb1 as [Hb1|Hb1]; [apply N.leb_gt in Hb1; lia | apply N.leb_gt in Hb1; lia].
+    + apply N.eqb_neq in Hb2. contradiction.
+Qed.
+
+(* Fixpoint that skips whitespace characters up to k bytes *)
+Fixpoint handle_whitespace (mem:memory) (p:addr) (k:nat) : addr :=
+  match k with
+  | O => p (* no more budget, return current position *)
+  | S k' => 
+    if is_whitespace_dec (mem Ⓑ[p])
+    then handle_whitespace mem (p ⊕ 1) k' (* skip whitespace, continue *)
+    else p (* found non-whitespace, stop *)
+  end.
